@prefix rdf: <http://www.w3.org/1999/02/22-rdf-syntax-ns#> .
@prefix rdfs: <http://www.w3.org/2000/01/rdf-schema#> .
@prefix xsd: <http://www.w3.org/2001/XMLSchema#> .
@prefix : <https://w3id.org/okp4/ontology/v$major/schema/credential/orchestration-service/execution/> .
@prefix schema: <http://schema.org/> .

:OrchestrationServiceExecution a rdfs:Class ;
  rdfs:label "Orchestration Service Execution"@en ;
  rdfs:comment """
  Captures the details of the progress and outcomes of the execution of an Orchestration Service.
  """@en .

:OrchestrationServiceExecutionCredential a rdfs:Class ;
  rdfs:label "Orchestration Service Execution Credential"@en ;
  rdfs:comment """
  A credential that provides proof of the execution of an Orchestration Service for a considered Orchestration Service Execution Order. It includes details of all the resources involved (consumed and produced), the time and date of execution, the parameters used, and any outcomes or results relevant to the execution.

  In these credentials, the Orchestration service is both the subject and the issuer.

  This credential is fundamental in providing a formal record of the execution of a digital service, which can be used for auditing, verification, and other purposes.
  """@en .

:executionOf a rdf:Property ;
  rdfs:label "execution of"@en ;
  rdfs:comment """
  This relationship is pivotal for associating the formal execution request with the corresponding credential, providing the necessary authorization and detailed directives for service execution. This ensures a verifiable and formalized process for initiating and tracking the execution of orchestration services.
  """@en ;
  schema:domainIncludes :OrchestrationServiceExecutionOrderCredential ;
  schema:rangeIncludes :OrchestrationServiceExecutionOrder .

:hasConsumedResource a rdf:Property ;
  rdfs:label "has consumed resource"@en ;
  rdfs:comment """
  Specifies a resource consumed during this Orchestration Service Execution. The resource can be any URI denoting a Digital Resource (such as a dataset), or a Digital Service (such as a Storage Service or a Processing Service).
  
  Multiple instances of `hasConsumedResource` can represent various resources consumed during the execution. Accessing a Digital Resource may require the use of multiple Digital Services, reflecting the complexity and interdependencies of digital service orchestration.
  """@en ;
  schema:domainIncludes :OrchestrationServiceExecution ;
  schema:rangeIncludes xsd:anyURI .

:hasExecution a rdf:Property ;
  rdfs:label "has execution result"@en ;
  rdfs:comment """
  The execution of the Orchestration Service.
  """@en ;
  schema:domainIncludes :OrchestrationServiceExecutionCredential ;
  schema:rangeIncludes :OrchestrationServiceExecution .

:hasExecutionStatus a rdf:Property ;
  rdfs:label "has execution status"@en ;
  rdfs:comment """
  Indicates the status of the service execution.
  """@en ;
  schema:domainIncludes :OrchestrationServiceExecutionCredential ;
  schema:rangeIncludes <https://w3id.org/okp4/ontology/v$major/thesaurus/digital-service-execution-status> .

:hasExecutionTime a rdf:Property ;
  rdfs:label "has execution time"@en ;
  rdfs:comment """
  The time and date when the Digital Service was executed.
  """@en ;
  schema:domainIncludes :OrchestrationServiceExecution ;
  schema:rangeIncludes schema:DateTime .

:hasProducedResource a rdf:Property ;
  rdfs:label "has produced resource"@en ;
  rdfs:comment """
  Specify a resource produced during this Orchestration Service Execution, if any. The resource can be any URI denoting a Digital Resource (such as a dataset), or a Digital Service (such as a Storage Service or a Processing Service).
  """@en ;
  schema:domainIncludes :OrchestrationServiceExecution ;
  schema:rangeIncludes xsd:anyURI .

:partOfExecution a rdf:Property ;
  rdfs:label "part of execution"@en ;
  rdfs:comment """
    Links an Orchestration Service Execution to its parent Orchestration Service Execution, if any.
    
    This property establishes a hierarchical relationship between executions, enabling the tracking of complex orchestration services composed of multiple, nested sub-executions. It enables the understanding the structure and progress of workflows that involve sequential or parallel steps.
  """@en ;
  schema:domainIncludes :OrchestrationServiceExecution ;
  schema:rangeIncludes :OrchestrationServiceExecution .


