@prefix rdf: <http://www.w3.org/1999/02/22-rdf-syntax-ns#> .
@prefix rdfs: <http://www.w3.org/2000/01/rdf-schema#> .
@prefix : <https://w3id.org/okp4/ontology/vnext/thesaurus/digital-service-execution-status/> .
@prefix dcterms: <http://purl.org/dc/terms/> .
@prefix skos: <http://www.w3.org/2004/02/skos/core#> .

:Cancelled a skos:Concept ;
  skos:definition """
  A term used to indicate that the execution of a Digital Service has been cancelled.
  """@en ;
  skos:inScheme <https://w3id.org/okp4/ontology/vnext/thesaurus/digital-service-execution-status> ;
  skos:prefLabel "Cancelled"@en .

:Delivered a skos:Concept ;
  skos:definition """
  A term used to indicate that the execution of a Digital Service has been completed and the service 
  has been delivered to the user.
  """@en ;
  skos:inScheme <https://w3id.org/okp4/ontology/vnext/thesaurus/digital-service-execution-status> ;
  skos:prefLabel "Delivered"@en .

:Failed a skos:Concept ;
  skos:definition """
  A term used to indicate that the execution of a Digital Service has failed.
  """@en ;
  skos:inScheme <https://w3id.org/okp4/ontology/vnext/thesaurus/digital-service-execution-status> ;
  skos:prefLabel "Failed"@en .

:InExecution a skos:Concept ;
  skos:definition """
  A term used to indicate that the execution of a Digital Service is currently in progress.
  """@en ;
  skos:inScheme <https://w3id.org/okp4/ontology/vnext/thesaurus/digital-service-execution-status> ;
  skos:prefLabel "In Execution"@en .

<https://w3id.org/okp4/ontology/vnext/thesaurus/digital-service-execution-status> a skos:ConceptScheme ;
  rdfs:label "Digital Service Execution Status Thesaurus"@en ;
  dcterms:description """
  This thesaurus defines a controlled vocabulary for representing the status of execution of Digital Services. This allows for standardized representation and understanding of execution status in various systems.
  """@en ;
  dcterms:title "The OKP4 Execution Status Thesaurus"@en .


