@prefix rdf: <http://www.w3.org/1999/02/22-rdf-syntax-ns#> .
@prefix rdfs: <http://www.w3.org/2000/01/rdf-schema#> .
@prefix xsd: <http://www.w3.org/2001/XMLSchema#> .
@prefix : <https://w3id.org/okp4/ontology/v3/schema/credential/digital-service/description/> .
@prefix schema: <http://schema.org/> .
@prefix thesaurus: <https://w3id.org/okp4/ontology/v3/thesaurus/> .

:DigitalServiceDescriptionCredential a rdfs:Class ;
  rdfs:label "Digital Service Description Credential"@en ;
  rdfs:comment """
  Digital Service Description credentials offer a comprehensive summary of a Digital Service's key features, encompassing aspects like its title, description, and associated tags. 

  Their primary function is to simplify the process for users to grasp the service's intent and practical application. 
  """@en .

:hasCategory a rdf:Property ;
  rdfs:label "has category"@en ;
  rdfs:comment """
  A category of the Digital Service.
  """@en ;
  schema:domainIncludes :DigitalServiceDescriptionCredential ;
  schema:rangeIncludes thesaurus:service-category .

:hasDescription a rdf:Property ;
  rdfs:label "has description"@en ;
  rdfs:comment """
  A description of the Digital Service.
  """@en ;
  schema:domainIncludes :DigitalServiceDescriptionCredential ;
  schema:rangeIncludes xsd:string .

:hasImage a rdf:Property ;
  rdfs:label "has image"@en ;
  rdfs:comment """
  The image associated with the Digital Service. 
  """@en ;
  schema:domainIncludes :DigitalServiceDescriptionCredential ;
  schema:rangeIncludes xsd:anyURI .

:hasPublisher a rdf:Property ;
  rdfs:label "has publisher"@en ;
  rdfs:comment """
  An entity primarily responsible for making the Digital Service available.
  """@en ;
  schema:domainIncludes :DigitalServiceDescriptionCredential ;
  schema:rangeIncludes schema:Organization ;
  schema:rangeIncludes schema:Person .

:hasTag a rdf:Property ;
  rdfs:label "has tag"@en ;
  rdfs:comment """
  A (free) keyword or term assigned to the Digital Service. 
  """@en ;
  schema:domainIncludes :DigitalServiceDescriptionCredential ;
  schema:rangeIncludes xsd:string .

:hasTitle a rdf:Property ;
  rdfs:label "has title"@en ;
  rdfs:comment """
  The title of the Digital Service.
  """@en ;
  schema:domainIncludes :DigitalServiceDescriptionCredential ;
  schema:rangeIncludes xsd:string .

:hasWebpage a rdf:Property ;
  rdfs:label "has webpage"@en ;
  rdfs:comment """
  A public web page detailing the service, its pricing and any other information useful for the user of the service.
  """@en ;
  schema:domainIncludes :DigitalServiceDescriptionCredential ;
  schema:rangeIncludes xsd:anyURI .


