@prefix rdf: <http://www.w3.org/1999/02/22-rdf-syntax-ns#> .
@prefix rdfs: <http://www.w3.org/2000/01/rdf-schema#> .
@prefix xsd: <http://www.w3.org/2001/XMLSchema#> .
@prefix owl: <http://www.w3.org/2002/07/owl#> .
@prefix dcterms: <http://purl.org/dc/terms/> .
@prefix okp4core: <https://ontology.okp4.space/core/> .
@prefix okp4th: <https://ontology.okp4.space/thesaurus/> .
@prefix skos: <http://www.w3.org/2004/02/skos/core#> .

okp4core:DIDURI a owl:Class ;
  rdfs:label "Decentralized Identifier URI"@en ;
  rdfs:comment "A decentralized identifier URI is a URI that identifies a subject in a decentralized system and is managed independently of any centralized registry."@en ;
  rdfs:seeAlso <https://www.w3.org/TR/did-core/> ;
  rdfs:subClassOf xsd:anyURI .

okp4core:Data a owl:Class ;
  rdfs:label "Data" ;
  rdfs:comment """
  `Data` denotes a quantity of information (processed or stored). 
  """@en .

okp4core:DataSpace a owl:Class ;
  rdfs:label "Data Space"@en ;
  rdfs:comment """
  `Data Space` is a founding concept of this ontology and is described as an abstraction that comprises:
  
  - Bundle of rights & rules that regulates interactions between data, algorithms, infrastructure and every resources shared by participants.
  - Governance mechanisms to adapt these rules.

  ![Data spaces](images/dataspace.png)

A Data Space is highly customizable to allow its members to create a space of sharing designed exactly as they need.
  """@en ;
  rdfs:subClassOf okp4core:Data .

okp4core:Dataset a owl:Class ;
  rdfs:label "Dataset"@en ;
  rdfs:comment """
  `Dataset` represents the group of related data that is organized and presented in a specific format by the provider. This data can take many forms, 
  including csv files, images, videos, and more, as well as data sources such as databases and APIs.

  Each dataset is identified and located by its unique [URI](https://en.wikipedia.org/wiki/Uniform_Resource_Identifier) which defines the path and 
  mean to access the data through the provider service.

  Datasets are described by a set of descriptions (aka metadata) providing information about one or more aspects of the dataset, like the
  time and date of creation, the file size or the data quality, using specific data description vocabularies and thesaurus (e.g. `Exif`, `EBUCore`, ISO 19115),
  allowing a great extensibility.
  """@en ;
  rdfs:subClassOf [
    a owl:Restriction ;
    owl:allValuesFrom okp4core:Service ;
    owl:onProperty okp4core:providedBy ;
  ] ;
  rdfs:subClassOf [
    a owl:Restriction ;
    owl:allValuesFrom okp4core:DIDURI ;
    owl:onProperty okp4core:hasRegistrar ;
  ] ;
  rdfs:subClassOf [
    a owl:Restriction ;
    owl:allValuesFrom xsd:anyURI ;
    owl:onProperty okp4core:hasIdentifier ;
  ] ;
  rdfs:subClassOf okp4core:Data .

okp4core:Metadata a owl:Class ;
  rdfs:label "Metadata"@en ;
  rdfs:comment """
  `Metadata` denotes the information data about `Data` (i.e. data about the data).
   """@en ;
  rdfs:subClassOf [
    a owl:Restriction ;
    owl:allValuesFrom okp4core:Data ;
    owl:onProperty okp4core:describes ;
  ] ;
  rdfs:subClassOf okp4core:Data .

okp4core:Period a owl:Class ;
  rdfs:label "Period"@en ;
  rdfs:comment """
  The Period class represents an interval of time, defined by a start and end time and date.
  """@en ;
  rdfs:subClassOf [
    a owl:Restriction ;
    owl:allValuesFrom xsd:dateTime ;
    owl:onProperty okp4core:hasStartDate ;
  ] ;
  rdfs:subClassOf [
    a owl:Restriction ;
    owl:minQualifiedCardinality "0"^^xsd:nonNegativeInteger ;
    owl:onDataRange xsd:dateTime ;
    owl:onProperty okp4core:hasEndDate ;
  ] .

okp4core:Resource a owl:Class ;
  rdfs:label "Resource"@en ;
  rdfs:comment """
  `Resource` denotes members of a `Data Space`, including datasets, services...
  """@en ;
  owl:unionOf ( okp4core:Dataset okp4core:Service ) ;
  rdfs:subClassOf [
    a owl:Restriction ;
    owl:allValuesFrom okp4core:DataSpace ;
    owl:onProperty okp4core:belongsTo ;
  ] .

okp4core:Service a owl:Class ;
  rdfs:label "Service"@en ;
  rdfs:comment """
  `Service` is a generic concept for any kind of service that can be provided through a network (e.g. a REST API, a gRPC service, etc.).

  Each service is identified and located by its unique [URI](https://en.wikipedia.org/wiki/Uniform_Resource_Identifier) which defines the entry point
  of the service.

  Services are described by a set of descriptions (aka metadata) providing information about one or more aspects of the service, like the purpose of the service,
  the general information of the provider, etc.
  """@en ;
  rdfs:subClassOf [
    a owl:Restriction ;
    owl:allValuesFrom xsd:anyURI ;
    owl:onProperty okp4core:hasIdentifier ;
  ] ;
  rdfs:subClassOf [
    a owl:Restriction ;
    owl:allValuesFrom okp4core:DIDURI ;
    owl:onProperty okp4core:hasIdentity ;
  ] ;
  rdfs:subClassOf [
    a owl:Restriction ;
    owl:allValuesFrom okp4core:DIDURI ;
    owl:onProperty okp4core:hasRegistrar ;
  ] ;
  rdfs:subClassOf okp4core:Data .

okp4core:belongsTo a owl:ObjectProperty ;
  rdfs:label "belongs to"@en ;
  rdfs:comment "Denotes the state of membership of an entity towards another."@en .

okp4core:describes a owl:ObjectProperty, owl:FunctionalProperty ;
  rdfs:label "describes"@en ;
  rdfs:comment "Description link between a resource (i.e. the data) and the description of that resource (i.e. metadata)."@en .

okp4core:hasCategory a owl:ObjectProperty, owl:FunctionalProperty ;
  rdfs:label "has category"@en ;
  rdfs:comment "A category of the resource."@en ;
  rdfs:range skos:Concept .

okp4core:hasIdentifier a owl:ObjectProperty, owl:FunctionalProperty ;
  rdfs:label "has identifier"@en ;
  rdfs:comment "An identifier for the resource."@en ;
  rdfs:range xsd:anyURI .

okp4core:hasIdentity a owl:ObjectProperty, owl:FunctionalProperty ;
  rdfs:label "has identity"@en ;
  rdfs:comment """
  The identity property represents the identity for a resource.
  """@en ;
  rdfs:range okp4core:DIDURI .

okp4core:hasImage a owl:ObjectProperty, owl:FunctionalProperty ;
  rdfs:label "has image"@en ;
  rdfs:comment "An image of the resource."@en ;
  rdfs:range xsd:anyURI .

okp4core:hasLicense a owl:ObjectProperty, owl:FunctionalProperty ;
  rdfs:label "has license"@en ;
  rdfs:comment "A legal document giving official permission to do something with the resource."@en ;
  rdfs:range okp4th:license .

okp4core:hasRegistrar a owl:ObjectProperty, owl:FunctionalProperty ;
  rdfs:label "has registrar"@en ;
  rdfs:comment "References the individual, company, or organization that is responsible for registering and managing a resource."@en ;
  rdfs:range okp4core:DIDURI .

okp4core:hasSpatialCoverage a owl:ObjectProperty, owl:FunctionalProperty ;
  rdfs:label "has spatial coverage"@en ;
  rdfs:comment "The spatial applicability of the resource."@en ;
  rdfs:range okp4th:area .

okp4core:hasTemporalCoverage a owl:ObjectProperty, owl:FunctionalProperty ;
  rdfs:label "has temporal coverage"@en ;
  rdfs:comment "The temporal applicability of the resource."@en ;
  rdfs:range okp4core:Period .

okp4core:hasTopic a owl:ObjectProperty, owl:FunctionalProperty ;
  rdfs:label "has topic"@en ;
  rdfs:comment "A topic of the resource."@en ;
  rdfs:range okp4th:topic .

okp4core:providedBy a owl:ObjectProperty, owl:FunctionalProperty ;
  rdfs:label "provided by"@en ;
  rdfs:comment "References the entity that provides the resource."@en ;
  rdfs:range xsd:anyURI .

okp4core:hasCreator a owl:DatatypeProperty, owl:FunctionalProperty ;
  rdfs:label "has creator"@en ;
  rdfs:comment "An entity primarily responsible for making the resource."@en ;
  rdfs:range xsd:string .

okp4core:hasDescription a owl:DatatypeProperty, owl:FunctionalProperty ;
  rdfs:label "has description"@en ;
  rdfs:comment """
  A human-readable description of the resource.
  """@en ;
  rdfs:range xsd:string .

okp4core:hasEndDate a owl:DatatypeProperty, owl:FunctionalProperty ;
  rdfs:label "has end date"@en ;
  rdfs:comment """
  The end date property represents the start date of an interval of time.
  """@en ;
  rdfs:range xsd:dateTime .

okp4core:hasPublisher a owl:DatatypeProperty, owl:FunctionalProperty ;
  rdfs:label "has publisher"@en ;
  rdfs:comment "An entity primarily responsible for making the resource available."@en ;
  rdfs:range xsd:string .

okp4core:hasStartDate a owl:DatatypeProperty, owl:FunctionalProperty ;
  rdfs:label "has start date"@en ;
  rdfs:comment """
  The start date property represents the start date of an interval of time.
  """@en ;
  rdfs:range xsd:dateTime .

okp4core:hasTag a owl:DatatypeProperty ;
  rdfs:label "has tag"@en ;
  rdfs:comment """
  A keyword or term assigned to the resource.
  """@en ;
  rdfs:range xsd:string .

okp4core:hasTitle a owl:DatatypeProperty, owl:FunctionalProperty ;
  rdfs:label "has title"@en ;
  rdfs:comment "A name given to the resource."@en ;
  rdfs:range xsd:string .

dcterms:description a owl:AnnotationProperty .

dcterms:title a owl:AnnotationProperty .

okp4core:wasCreatedBy a owl:AnnotationProperty ;
  rdfs:label "was created by"@en ;
  rdfs:comment """
  Information about who created the resource.

  This information is stored initially and will never be changed thereafter.
  """@en ;
  rdfs:range xsd:uri .


