@prefix rdf: <http://www.w3.org/1999/02/22-rdf-syntax-ns#> .
@prefix rdfs: <http://www.w3.org/2000/01/rdf-schema#> .
@prefix xsd: <http://www.w3.org/2001/XMLSchema#> .
@prefix owl: <http://www.w3.org/2002/07/owl#> .
@prefix dcterms: <http://purl.org/dc/terms/> .
@prefix okp4core: <https://ontology.okp4.space/core/> .
@prefix okp4th: <https://ontology.okp4.space/thesaurus/> .
@prefix skos: <http://www.w3.org/2004/02/skos/core#> .

okp4core:DIDURI a owl:Class ;
  rdfs:label "Decentralized Identifier URI"@en ;
  rdfs:comment "A decentralized identifier URI is a URI that identifies a subject in a decentralized system and is managed independently of any centralized registry."@en ;
  rdfs:seeAlso <https://www.w3.org/TR/did-core/> ;
  rdfs:subClassOf xsd:anyURI .

okp4core:Data a owl:Class ;
  rdfs:label "Data" ;
  rdfs:comment """
  `Data` denotes a quantity of information (processed or stored). 
  """@en .

okp4core:DataSpace a owl:Class ;
  rdfs:label "Data Space"@en ;
  rdfs:comment """
  `Data Space` is a founding concept of this ontology and is described as an abstraction that comprises:
  
  - Bundle of rights & rules that regulates interactions between data, algorithms, infrastructure and every resources shared by participants.
  - Governance mechanisms to adapt these rules.

  ![Data spaces](images/dataspace.png)

A Data Space is highly customizable to allow its members to create a space of sharing designed exactly as they need.
  """@en ;
  rdfs:subClassOf [
    a owl:Restriction ;
    owl:allValuesFrom okp4core:DIDURI ;
    owl:onProperty okp4core:hasRegistrar ;
  ] .

okp4core:Dataset a owl:Class ;
  rdfs:label "Dataset"@en ;
  rdfs:comment """
  `Dataset` represents the group of related data that is organized and presented in a specific format by the provider. This data can take many forms, 
  including csv files, images, videos, and more, as well as data sources such as databases and APIs.

  Each dataset is identified and located by its unique [URI](https://en.wikipedia.org/wiki/Uniform_Resource_Identifier) which defines the path and 
  mean to access the data through the provider service.

  Datasets are described by a set of descriptions (aka metadata) providing information about one or more aspects of the dataset, like the
  time and date of creation, the file size or the data quality, using specific data description vocabularies and thesaurus (e.g. `Exif`, `EBUCore`, ISO 19115),
  allowing a great extensibility.
  """@en ;
  rdfs:subClassOf [
    a owl:Restriction ;
    owl:allValuesFrom okp4core:DIDURI ;
    owl:onProperty okp4core:hasRegistrar ;
  ] ;
  rdfs:subClassOf [
    a owl:Restriction ;
    owl:allValuesFrom okp4core:Service ;
    owl:onProperty okp4core:providedBy ;
  ] ;
  rdfs:subClassOf [
    a owl:Restriction ;
    owl:allValuesFrom xsd:anyURI ;
    owl:onProperty okp4core:hasIdentifier ;
  ] .

okp4core:Governance a owl:Class ;
  rdfs:label "Governance"@en ;
  rdfs:comment """
    `Governance` is a set of rules that define how a `Data Space` is managed and how the resources are shared.
  """@en ;
  rdfs:subClassOf [
    a owl:Restriction ;
    owl:allValuesFrom xsd:anyURI ;
    owl:onProperty okp4core:hasIdentifier ;
  ] ;
  rdfs:subClassOf [
    a owl:Restriction ;
    owl:allValuesFrom okp4core:DIDURI ;
    owl:onProperty okp4core:hasRegistrar ;
  ] .

okp4core:Metadata a owl:Class ;
  rdfs:label "Metadata"@en ;
  rdfs:comment """
  `Metadata` denotes the information data about `Data` (i.e. data about the data).
   """@en ;
  rdfs:subClassOf [
    a owl:Restriction ;
    owl:allValuesFrom okp4core:Data ;
    owl:onProperty okp4core:describes ;
  ] .

okp4core:Period a owl:Class ;
  rdfs:label "Period"@en ;
  rdfs:comment """
  The Period class represents an interval of time, defined by a start and end time and date.
  """@en ;
  rdfs:subClassOf [
    a owl:Restriction ;
    owl:minQualifiedCardinality "0"^^xsd:nonNegativeInteger ;
    owl:onDataRange xsd:dateTime ;
    owl:onProperty okp4core:hasEndDate ;
  ] ;
  rdfs:subClassOf [
    a owl:Restriction ;
    owl:allValuesFrom xsd:dateTime ;
    owl:onProperty okp4core:hasStartDate ;
  ] .

okp4core:Resource a owl:Class ;
  rdfs:label "Resource"@en ;
  rdfs:comment """
  `Resource` denotes members of a `Data Space`, including datasets, services...
  """@en ;
  owl:unionOf ( okp4core:Dataset okp4core:Service okp4core:Governance ) ;
  rdfs:subClassOf [
    a owl:Restriction ;
    owl:allValuesFrom okp4core:DataSpace ;
    owl:onProperty okp4core:belongsTo ;
  ] .

okp4core:Service a owl:Class ;
  rdfs:label "Service"@en ;
  rdfs:comment """
  `Service` is a generic concept for any kind of service that can be provided through a network (e.g. a REST API, a gRPC service, etc.).

  Each service is identified and located by its unique [URI](https://en.wikipedia.org/wiki/Uniform_Resource_Identifier) which defines the entry point
  of the service.

  Services are described by a set of descriptions (aka metadata) providing information about one or more aspects of the service, like the purpose of the service,
  the general information of the provider, etc.
  """@en ;
  rdfs:subClassOf [
    a owl:Restriction ;
    owl:allValuesFrom okp4core:DIDURI ;
    owl:onProperty okp4core:hasIdentity ;
  ] ;
  rdfs:subClassOf [
    a owl:Restriction ;
    owl:allValuesFrom xsd:anyURI ;
    owl:onProperty okp4core:hasIdentifier ;
  ] ;
  rdfs:subClassOf [
    a owl:Restriction ;
    owl:allValuesFrom okp4core:DIDURI ;
    owl:onProperty okp4core:hasRegistrar ;
  ] .

okp4core:ServiceExecution a owl:Class ;
  rdfs:label "Service Execution"@en ;
  rdfs:comment """
     The execution of a service with specific inputs and outputs. It represents the actual execution of a service in a ServiceExecutionOrder, along with its 
     input and output datasets and metadata.
  """@en ;
  owl:equivalentClass [
    a owl:Class ;
    owl:intersectionOf ( [
      a owl:Restriction ;
      owl:allValuesFrom okp4core:Service ;
      owl:onProperty okp4core:hasObject ;
    ] [
      a owl:Class ;
      owl:unionOf ( [
        a owl:Restriction ;
        owl:allValuesFrom okp4core:Dataset ;
        owl:onProperty okp4core:produces ;
      ] [
        a owl:Restriction ;
        owl:allValuesFrom okp4core:Metadata ;
        owl:onProperty okp4core:produces ;
      ] ) ;
    ] [
      a owl:Restriction ;
      owl:allValuesFrom okp4core:Dataset ;
      owl:onProperty okp4core:hasInput ;
    ] [
      a owl:Restriction ;
      owl:allValuesFrom okp4core:ServiceExecutionOrder ;
      owl:onProperty okp4core:specifiedBy ;
    ] [
      a owl:Restriction ;
      owl:allValuesFrom okp4core:ServiceExecution ;
      owl:onProperty okp4core:hasParent ;
    ] ) ;
  ] .

okp4core:ServiceExecutionOrder a owl:Class ;
  rdfs:label "Service Execution Order"@en ;
  rdfs:comment """
    Formal representation of the order in which services should be executed. To specify the details of a service execution, such as the required resources 
    (datasets), expected results, and potential time considerations, metadata should be used.
    """@en ;
  owl:equivalentClass [
    a owl:Class ;
    owl:intersectionOf ( [
      a owl:Restriction ;
      owl:allValuesFrom okp4core:DIDURI ;
      owl:onProperty okp4core:hasContractingParty ;
    ] [
      a owl:Restriction ;
      owl:allValuesFrom okp4core:Service ;
      owl:onProperty okp4core:hasContractor ;
    ] [
      a owl:Restriction ;
      owl:allValuesFrom okp4core:Service ;
      owl:onProperty okp4core:hasObject ;
    ] ) ;
  ] .

okp4core:belongsTo a owl:ObjectProperty ;
  rdfs:label "belongs to"@en ;
  rdfs:comment "Denotes the state of membership of an entity towards another."@en .

okp4core:createdBy a owl:ObjectProperty ;
  rdfs:label "created by"@en ;
  rdfs:comment """
  The entity who created the resource.
  """@en ;
  rdfs:range okp4core:DIDURI .

okp4core:describes a owl:ObjectProperty, owl:FunctionalProperty ;
  rdfs:label "describes"@en ;
  rdfs:comment "Description link between a resource (i.e. the data) and the description of that resource (i.e. metadata)."@en .

okp4core:hasCategory a owl:ObjectProperty, owl:FunctionalProperty ;
  rdfs:label "has category"@en ;
  rdfs:comment "A category of the resource."@en ;
  rdfs:range skos:Concept .

okp4core:hasContractingParty a owl:ObjectProperty ;
  rdfs:label "has contracting party"@en ;
  rdfs:comment "Link to the contracting party, identified by a decentralized identifier (DID)."@en ;
  rdfs:range okp4core:DIDURI .

okp4core:hasContractor a owl:ObjectProperty ;
  rdfs:label "has contractor"@en ;
  rdfs:comment "Link to the contractor responsible for executing a work on a contract basis."@en .

okp4core:hasFormat a owl:ObjectProperty, owl:FunctionalProperty ;
  rdfs:label "has format"@en ;
  rdfs:comment "The format of the resource."@en ;
  rdfs:range skos:Concept .

okp4core:hasIdentifier a owl:ObjectProperty, owl:FunctionalProperty ;
  rdfs:label "has identifier"@en ;
  rdfs:comment "An identifier for the resource."@en ;
  rdfs:range xsd:anyURI .

okp4core:hasIdentity a owl:ObjectProperty, owl:FunctionalProperty ;
  rdfs:label "has identity"@en ;
  rdfs:comment """
  The identity property represents the identity for a resource.
  """@en ;
  rdfs:range okp4core:DIDURI .

okp4core:hasImage a owl:ObjectProperty, owl:FunctionalProperty ;
  rdfs:label "has image"@en ;
  rdfs:comment "An image of the resource."@en ;
  rdfs:range xsd:anyURI .

okp4core:hasInput a owl:ObjectProperty ;
  rdfs:label "has input"@en ;
  rdfs:comment "Specifies a resource which acts as an input."@en .

okp4core:hasLicense a owl:ObjectProperty, owl:FunctionalProperty ;
  rdfs:label "has license"@en ;
  rdfs:comment "A legal document giving official permission to do something with the resource."@en ;
  rdfs:range okp4th:license .

okp4core:hasParent a owl:ObjectProperty ;
  rdfs:label "has parent"@en ;
  rdfs:comment "describe the relationship between two resources, where one resource is the parent of another resource."@en .

okp4core:hasRegistrar a owl:ObjectProperty, owl:FunctionalProperty ;
  rdfs:label "has registrar"@en ;
  rdfs:comment "References the individual, company, or organization that is responsible for registering and managing a resource."@en ;
  rdfs:range okp4core:DIDURI .

okp4core:hasSpatialCoverage a owl:ObjectProperty, owl:FunctionalProperty ;
  rdfs:label "has spatial coverage"@en ;
  rdfs:comment "The spatial applicability of the resource."@en ;
  rdfs:range okp4th:area .

okp4core:hasTemporalCoverage a owl:ObjectProperty, owl:FunctionalProperty ;
  rdfs:label "has temporal coverage"@en ;
  rdfs:comment "The temporal applicability of the resource."@en ;
  rdfs:range okp4core:Period .

okp4core:hasTopic a owl:ObjectProperty, owl:FunctionalProperty ;
  rdfs:label "has topic"@en ;
  rdfs:comment "A topic of the resource."@en ;
  rdfs:range skos:Concept .

okp4core:hasObject a owl:ObjectProperty ;
  rdfs:label "has object"@en ;
  rdfs:comment "Express the relationship between two resources where the second one is related to, or included in, the first one in some way."@en .

okp4core:lastModifiedBy a owl:ObjectProperty ;
  rdfs:label "last modified by"@en ;
  rdfs:comment """
  The entity who last modified the resource.
  """@en ;
  rdfs:range okp4core:DIDURI .

okp4core:produces a owl:ObjectProperty, owl:FunctionalProperty ;
  rdfs:label "produces"@en ;
  rdfs:comment "Specifies a resource which is produced."@en .

okp4core:providedBy a owl:ObjectProperty, owl:FunctionalProperty ;
  rdfs:label "provided by"@en ;
  rdfs:comment "References the entity that provides the resource."@en ;
  rdfs:range xsd:anyURI .

okp4core:specifiedBy a owl:ObjectProperty ;
  rdfs:label "specified by"@en ;
  rdfs:comment "Reference the resource which specify clearly, exactly this resource."@en .

okp4core:createdOn a owl:DatatypeProperty ;
  rdfs:label "created on"@en ;
  rdfs:comment """
  The date and time when the resource was created.
  """@en ;
  rdfs:range xsd:dateTime .

okp4core:hasCreator a owl:DatatypeProperty, owl:FunctionalProperty ;
  rdfs:label "has creator"@en ;
  rdfs:comment "An entity primarily responsible for making the resource."@en ;
  rdfs:range xsd:string .

okp4core:hasDescription a owl:DatatypeProperty, owl:FunctionalProperty ;
  rdfs:label "has description"@en ;
  rdfs:comment """
  A human-readable description of the resource.
  """@en ;
  rdfs:range xsd:string .

okp4core:hasEndDate a owl:DatatypeProperty, owl:FunctionalProperty ;
  rdfs:label "has end date"@en ;
  rdfs:comment """
  The end date property represents the start date of an interval of time.
  """@en ;
  rdfs:range xsd:dateTime .

okp4core:hasPublisher a owl:DatatypeProperty, owl:FunctionalProperty ;
  rdfs:label "has publisher"@en ;
  rdfs:comment "An entity primarily responsible for making the resource available."@en ;
  rdfs:range xsd:string .

okp4core:hasStartDate a owl:DatatypeProperty, owl:FunctionalProperty ;
  rdfs:label "has start date"@en ;
  rdfs:comment """
  The start date property represents the start date of an interval of time.
  """@en ;
  rdfs:range xsd:dateTime .

okp4core:hasTag a owl:DatatypeProperty ;
  rdfs:label "has tag"@en ;
  rdfs:comment """
  A keyword or term assigned to the resource.
  """@en ;
  rdfs:range xsd:string .

okp4core:hasTitle a owl:DatatypeProperty, owl:FunctionalProperty ;
  rdfs:label "has title"@en ;
  rdfs:comment "A name given to the resource."@en ;
  rdfs:range xsd:string .

okp4core:lastModifiedOn a owl:DatatypeProperty ;
  rdfs:label "last modified on"@en ;
  rdfs:comment """
  The date and time when the resource was last modified.
  """@en ;
  rdfs:range xsd:dateTime .

dcterms:description a owl:AnnotationProperty .

dcterms:title a owl:AnnotationProperty .


