@prefix rdfs: <http://www.w3.org/2000/01/rdf-schema#> .
@prefix xsd: <http://www.w3.org/2001/XMLSchema#> .
@prefix owl: <http://www.w3.org/2002/07/owl#> .
@prefix core: <https://ontology.okp4.space/core/> .
@prefix meta: <https://ontology.okp4.space/metadata/governance/> .

meta:Article a owl:Class ;
  rdfs:label "Article"@en ;
  rdfs:comment """
    An article of a governance text, which states a specific (legal) rule or principle. Articles are the smallest unit of a governance text which represents a significant rule that can be enforced. 
  """@en ;
  rdfs:subClassOf [
    a owl:Restriction ;
    owl:allValuesFrom xsd:string ;
    owl:onProperty core:hasTitle ;
  ] ;
  rdfs:subClassOf [
    a owl:Restriction ;
    owl:allValuesFrom meta:Subsection ;
    owl:onProperty core:isPartOf ;
  ] ;
  rdfs:subClassOf [
    a owl:Restriction ;
    owl:allValuesFrom xsd:string ;
    owl:onProperty meta:hasNumber ;
  ] ;
  rdfs:subClassOf [
    a owl:Restriction ;
    owl:allValuesFrom xsd:string ;
    owl:onProperty core:hasDescription ;
  ] .

meta:Chapter a owl:Class ;
  rdfs:label "Chapter"@en ;
  rdfs:comment "A chapter of a governance text, which groups related sections together."@en ;
  rdfs:subClassOf [
    a owl:Restriction ;
    owl:allValuesFrom xsd:string ;
    owl:onProperty core:hasTitle ;
  ] ;
  rdfs:subClassOf [
    a owl:Restriction ;
    owl:allValuesFrom xsd:string ;
    owl:onProperty core:hasDescription ;
  ] .

meta:GovernanceMetadata a owl:Class ;
  rdfs:label "Governance metadata"@en ;
  rdfs:comment """
    Governance Metadata provides descriptive information about a governance text. This metadata is distinct from the governance text itself, but helps to understand the governance text 
    by providing important context. The metadata describes the governance text in a hierarchical manner, organized into chapters, sections, and articles. This hierarchy helps to structure the governance text and makes it easier to navigate and comprehend.

    This metadata is especially valuable in decentralized applications and web3 interfaces where governance texts are utilized to describe and represent the rules governing Zones. This enables users to more readily engage with the governance text, allowing them to gain a better understanding of how the text operates and the rules governing the relationship between all resources within the Zones.
  """@en ;
  rdfs:subClassOf [
    a owl:Restriction ;
    owl:allValuesFrom meta:Chapter ;
    owl:onProperty meta:hasChapter ;
  ] ;
  rdfs:subClassOf [
    a owl:Restriction ;
    owl:allValuesFrom xsd:dateTime ;
    owl:onProperty core:createdOn ;
  ] ;.

meta:Paragraph a owl:Class ;
  rdfs:label "Paragraph"@en ;
  rdfs:comment """
    A paragraph of an article, which expresses a sub-rule or sub-principle of the article.
  """@en ;
  rdfs:subClassOf [
    a owl:Restriction ;
    owl:allValuesFrom xsd:string ;
    owl:onProperty core:hasTitle ;
  ] ;
  rdfs:subClassOf [
    a owl:Restriction ;
    owl:allValuesFrom xsd:string ;
    owl:onProperty meta:hasNumber ;
  ] ;
  rdfs:subClassOf [
    a owl:Restriction ;
    owl:allValuesFrom meta:Article ;
    owl:onProperty core:isPartOf ;
  ] ;
  rdfs:subClassOf [
    a owl:Restriction ;
    owl:allValuesFrom xsd:string ;
    owl:onProperty core:hasDescription ;
  ] .

meta:Section a owl:Class ;
  rdfs:label "Section"@en ;
  rdfs:comment "A section of a governance text, which groups related subsections together."@en ;
  rdfs:subClassOf [
    a owl:Restriction ;
    owl:allValuesFrom meta:Chapter ;
    owl:onProperty core:isPartOf ;
  ] ;
  rdfs:subClassOf [
    a owl:Restriction ;
    owl:allValuesFrom xsd:string ;
    owl:onProperty core:hasTitle ;
  ] ;
  rdfs:subClassOf [
    a owl:Restriction ;
    owl:allValuesFrom xsd:string ;
    owl:onProperty core:hasDescription ;
  ] ;
  rdfs:subClassOf [
    a owl:Restriction ;
    owl:allValuesFrom xsd:string ;
    owl:onProperty meta:hasNumber ;
  ] .

meta:Subsection a owl:Class ;
  rdfs:label "Subsection"@en ;
  rdfs:comment "A subsection of a governance text, which groups related articles together within a section."@en ;
  rdfs:subClassOf [
    a owl:Restriction ;
    owl:allValuesFrom meta:Section ;
    owl:onProperty core:isPartOf ;
  ] ;
  rdfs:subClassOf [
    a owl:Restriction ;
    owl:allValuesFrom xsd:string ;
    owl:onProperty meta:hasNumber ;
  ] ;
  rdfs:subClassOf [
    a owl:Restriction ;
    owl:allValuesFrom xsd:string ;
    owl:onProperty core:hasTitle ;
  ] ;
  rdfs:subClassOf [
    a owl:Restriction ;
    owl:allValuesFrom xsd:string ;
    owl:onProperty core:hasDescription ;
  ] .

meta:hasNumber a owl:DatatypeProperty, owl:FunctionalProperty ;
  rdfs:label "has number"@en ;
  rdfs:comment """
  A property that links a governance concept to its number.
  
  The value of the property is presented as a string, to allow for different numbering styles, such as Roman numerals or decimal numbers 
  with sub-numbers, like '1.2'.
  """@en ;
  rdfs:range xsd:string .


