@prefix owl: <http://www.w3.org/2002/07/owl#> .
@prefix dcterms: <http://purl.org/dc/terms/> .
@prefix xsd: <http://www.w3.org/2001/XMLSchema#> .
@prefix rdfs: <http://www.w3.org/2000/01/rdf-schema#> .
@prefix vann: <http://purl.org/vocab/vann/> .
@prefix vs: <http://www.w3.org/2003/06/sw-vocab-status/ns#> .

<https://ontology.okp4.com/core>
  a owl:Ontology ;
  owl:versionIRI <https://ontology.okp4.com/core/1.0.0> ;
  owl:versionInfo "v1.0.0" ;
  dcterms:created "2021-10-11"^^xsd:date ;
  dcterms:language "EN" ;
  dcterms:title "OKP4 Ontology: Ontology for Knowledge Graph"@en ;
  dcterms:license <https://creativecommons.org/licenses/by-sa/4.0/> ;
  dcterms:publisher <https://okp4.com/> ;
  dcterms:description """

  A vocabulary to describe knowledge graphs within dataspaces.

  This ontology is intended to model a semantic network of all the entities (datasets, services, actors...) of a dataspace by semantically characterizing 
  what they are and the relationships they maintain between them.
  
  The primary objective of the ontology is to provide a complete living understanding and knowledge of the datasets within a dataspace,
  their transformation (by the services), as well as the governance rules that apply (data sharing, consents, policy rules).  It also describes the 
  [Chain of Custody](https://en.wikipedia.org/wiki/Chain_of_custody) providing the Data Lineage (allowing the traceability) of each piece of data in the dataspaces during the 
  different processing.
"""@en ;
  rdfs:label "OKP4 Ontology"@en ;
  vann:preferredNamespacePrefix "okp4" ;
  vann:preferredNamespaceUri "https://ontology.okp4.com/core" ;
  vs:term_status "unstable"@en .

# -- annotation properties

dcterms:description a
  owl:AnnotationProperty .

dcterms:title a
  owl:AnnotationProperty .

# -- classes

<https://ontology.okp4.com/core/Dataspace>
  a rdfs:Class ;
  rdfs:label "Dataspace"@en ;
  rdfs:comment """
  
  `Dataspace` is a founding concept of this ontology and is described as a *virtual* space in which several entities belong (for instance datasets, services and actors), and
   governed by a set of explicit rules between all of them.
   
  """@en .

# -- properties

<https://ontology.okp4.com/core/hasName>
  a owl:FunctionalProperty, owl:DatatypeProperty ;
  rdfs:subPropertyOf dcterms:title ;
  rdfs:label "has name"@en ;
  rdfs:domain <https://ontology.okp4.com/core/Dataspace> ;
  rdfs:range xsd:string ;
  rdfs:comment "A name given to the resource."@en .

<https://ontology.okp4.com/core/hasDescription>
  a owl:FunctionalProperty, owl:DatatypeProperty ;
  rdfs:subPropertyOf dcterms:description ;
  rdfs:label "has description"@en ;
  rdfs:domain <https://ontology.okp4.com/core/Dataspace> ;
  rdfs:range xsd:string ;
  rdfs:comment """
  
  A short text description given to a resource.

  [Markdown](https://en.wikipedia.org/wiki/Markdown) syntax can be used for creating formatted text. 
  
  """@en .

<https://ontology.okp4.com/core/wasCreatedOn>
  a owl:FunctionalProperty, owl:DatatypeProperty ;
  rdfs:label "was created on"@en ;
  rdfs:domain <https://ontology.okp4.com/core/Dataspace> ;
  rdfs:range xsd:date ;
  rdfs:comment """

  Information on when the resource was created.
  
  This information is stored initially and will never be changed thereafter.

"""@en .

<https://ontology.okp4.com/core/wasCreatedBy>
  a owl:FunctionalProperty, owl:ObjectProperty ;
  rdfs:label "was created by"@en ;
  rdfs:domain <https://ontology.okp4.com/core/Dataspace> ;
  rdfs:range xsd:uri ;
  rdfs:comment """

  Information about who created the resource.
  
  This information is stored initially and will never be changed thereafter.

"""@en .
