@prefix rdf: <http://www.w3.org/1999/02/22-rdf-syntax-ns#> .
@prefix rdfs: <http://www.w3.org/2000/01/rdf-schema#> .
@prefix : <https://w3id.org/okp4/ontology/v3/schema/credential/digital-resource/rights/> .
@prefix schema: <http://schema.org/> .

:DigitalResourceRightsCredential a rdfs:Class ;
  rdfs:label "Digital Resource Rights Credential"@en ;
  rdfs:comment """
  Digital Resource Rights Credentials provide comprehensive information regarding the authorship, creation, publishing, and licensing of a Digital Resource.
  
  These details are critical for understanding the Digital Resource's provenance, ownership, and the terms under which it can be used.
  """@en .

:hasAuthor a rdf:Property ;
  rdfs:label "has author"@en ;
  rdfs:comment "The author(s) of the Digital Resource."@en ;
  schema:domainIncludes :DigitalResourceRightsCredential ;
  schema:rangeIncludes schema:Organization ;
  schema:rangeIncludes schema:Person .

:hasCreator a rdf:Property ;
  rdfs:label "has creator"@en ;
  rdfs:comment "The creator or entity responsible for compiling or generating the Digital Resource."@en ;
  schema:domainIncludes :DigitalResourceRightsCredential ;
  schema:rangeIncludes schema:Organization ;
  schema:rangeIncludes schema:Person .

:hasLicense a rdf:Property ;
  rdfs:label "has license"@en ;
  rdfs:comment "The licensing terms under which the Digital Resource is made available."@en ;
  schema:domainIncludes :DigitalResourceRightsCredential ;
  schema:rangeIncludes <https://w3id.org/okp4/ontology/v3/thesaurus/license> .

:hasPublisher a rdf:Property ;
  rdfs:label "has publisher"@en ;
  rdfs:comment "The publisher of the Digital Resource."@en ;
  schema:domainIncludes :DigitalResourceRightsCredential ;
  schema:rangeIncludes schema:Organization ;
  schema:rangeIncludes schema:Person .


