@prefix rdf: <http://www.w3.org/1999/02/22-rdf-syntax-ns#> .
@prefix rdfs: <http://www.w3.org/2000/01/rdf-schema#> .
@prefix xsd: <http://www.w3.org/2001/XMLSchema#> .
@prefix : <https://ontology.okp4.space/schema/credential/digital-resource/declaration/> .
@prefix schema: <http://schema.org/> .

:DigitalResourceDeclarationCredential a rdfs:Class ;
  rdfs:label "Digital Resource Declaration Credential"@en ;
  rdfs:comment """
  Digital Resource credentials serve as a testament to the declaration of a Digital Resource within the dataverse.
  
  Digital Resources serve as the raw material from which insights and new knowledge are extracted. They encompass data and information presented in various forms and expressed, carried, and stored in any format. This includes, but is not limited to spreadsheets, CSV fikes, databases, text documents, multimedia files such as videos, AI related files like neural network models, and various other digital elements.
  
  This concept is inherently flexible, adapting continuously to emerging digital formats and technological developments.
  """@en .

:hasIdentifier a rdf:Property ;
  rdfs:label "has identifier"@en ;
  rdfs:comment """
  The URI that identifies the resource.

  This URI makes sense only in the context of the Digital Service that provides the resource.
  """@en ;
  schema:domainIncludes :DigitalResourceDeclarationCredential ;
  schema:rangeIncludes xsd:anyURI .

:servedBy a rdf:Property ;
  rdfs:label "served by"@en ;
  rdfs:comment """
  The Digital Service that served the resource.

  This information is required to enable the interaction with the resource.

  In that sense Digital Services function as channels for the distribution and exchange of these Digital Resources across assorted networks. These services take various forms, including network communication protocols like RESTful APIs and gRPC services. They are pivotal in linking the resources with Orchestrator Services that utilize these resources for diverse applications.
  
  For instance, a Digital Resource may be a dataset that is accessed through a RESTful API, and is used by an Orchestrator Service to train a machine learning model.
  """@en ;
  schema:domainIncludes :DigitalResourceDeclarationCredential ;
  schema:rangeIncludes xsd:anyURI .


